ok
git-svn-id: svn://scm.gforge.inria.fr/svn/cfml@10 ba02c806-7d2b-4818-9a48-35b22e6bdc79

okasaki/ImplicitQueue_proof.v
@@ -1,29 +1,34 @@
 Set Implicit Arguments.
 Require Import FuncTactics LibCore.
 Require Import QueueSig_ml QueueSig_proof.
-Require Import BatchedQueue_ml.
+Require Import ImplicitQueue_ml.
 
-Module BatchedQueueSpec <: QueueSigSpec.
+Module ImplicitQueueSpec <: QueueSigSpec.
 
 (** instantiations *)
 
-Module Import Q <: MLQueue := MLBatchedQueue.
-Import MLBatchedQueue.
+Module Import Q <: MLQueue := MLImplicitQueue.
+Import MLImplicitQueue.
 
 (** invariant *)
 
 Global Instance queue_rep `{Rep a_ A} : Rep (queue a_) (list A) :=
-  fun (q:queue a_) (Q:list A) =>
-  let (f,r) := q in 
+  fun (q:queue a_) (Q:list A) => Q = nil.
+  (*let (f,r) := q in 
      Forall2 rep (f ++ rev r) Q
-  /\ (f = nil -> r = nil).
+  /\ (f = nil -> r = nil).*)
+
+  (*todo: xisspec loop is invariant is just true *)
 
 (** automation *)
 
 Hint Constructors Forall2.
 Hint Resolve Forall2_last.
 Hint Unfold is_head is_tail.
+(*
 Hint Extern 1 (@rep (queue _) _ _ _ _) => simpl; rew_list.
+Hint Extern 1 (@rep (queues _) _ _ _ _) => simpl; rew_list.
+*)
 
 Ltac auto_star ::= try solve [ rew_list in *; intuition (eauto) ].
 
@@ -31,6 +36,63 @@ Ltac auto_star ::= try solve [ rew_list in *; intuition (eauto) ].
 (** useful facts *)
 
 (** verification *)
+
+Definition spec_hyp_2 (A1 A2 B : Type)
+  (P:A1->A2->Prop) (K:A1->A2->~~B->Prop) f :=
+  spec_2 (fun x1 x2 R => P x1 x2 -> K x1 x2 R) f.
+
+(*
+Lemma spec_hyp_size : forall (A1 A2 : Type) (mu:A1->A2->nat) (B : Type)
+  (P:A1->A2->Prop) (K:A1->A2->~~B->Prop) f,
+  is_spec
+  (forall n, spec_hyp_2 (fun x1 x2 => n = mu x1 x2) K f) ->
+  spec_2 K f.
+*)
+
+Ltac xintros_core cont1 cont2 cont3 ::=
+   let arity := spec_goal_arity tt in
+   let lemma := get_spec_intro_x arity in
+   apply lemma; [ instantiate; cont1 tt | instantiate; cont2 tt | instantiate; cont3 tt ]. 
+
+Ltac xcurried_core ::=
+  let arity := spec_goal_arity tt in
+  let lemma := get_curried_prove_x arity in
+  eapply lemma; try solve [ xcf; auto; instantiate; try xisspec ].
+
+Lemma good_induct : forall (P : (nat->Prop) -> Prop),
+  (forall n, (forall m, n > m -> P (eq m)) -> P (gt n)) ->
+  (forall n, P (gt n) -> P (eq n)) ->
+  (forall n, P (eq n)).
+Proof. intros. induction n using peano_induction. auto. Qed. 
+
+Ltac name_around e x :=
+  pattern e; match goal with |- ?P _ => sets x: P end.
+
+Ltac xcf_for_core f ::=
+ ltac_database_get database_cf f;
+  let H := fresh "TEMP" in intros H; 
+  match type of H with
+  | tag tag_topfun _ _ => sapply H; [ instantiate; try xisspec | ]
+  | _ => sapply H
+  end; clear H; xcf_post tt.
+
+Lemma snoc_spec : forall `{Rep a A},
+  RepTotal snoc (Q;queue a) (X;a) >> (Q & X) ; queue a.
+Proof.
+  intros. xintros. intros. sets_eq n: (length Q). gen x1 x2 Q X.
+  gen H. gen a A. apply~ good_induct; clears n.
+  introv IH RQ N RX. subst_hyp N.
+  xcf_app; auto. xisspec. (* todo: automate xisspec *)
+  xmatch.
+  
+Qed.
+
+Hint Extern 1 (RegisterSpec snoc) => Provide snoc_spec.
+
+
+
+
+
 
 Section Polymorphic.
 Variables (a_ A : Type) (RA:Rep a_ A).
@@ -100,4 +162,4 @@ Hint Extern 1 (RegisterSpec tail) => Provide tail_spec.
 
 End Polymorphic.
 
-End BatchedQueueSpec.
+End ImplicitQueueSpec.
