go.sh
@@ -1,0 +1,1 @@
+coqide -I lib $1
